investigations/bedrock2/WhileProperties.v
@@ -1,0 +1,63 @@
+Require Import Coq.Lists.List.
+Require Import Coq.ZArith.ZArith.
+Require Import bedrock2.Semantics.
+Require Import bedrock2.Syntax.
+Require Import bedrock2.ProgramLogic.
+Require Import bedrock2.WeakestPrecondition.
+Require Import bedrock2.WeakestPreconditionProperties.
+Require Import coqutil.Word.Interface.
+Require Import coqutil.Word.Properties.
+Require Import coqutil.Map.Interface.
+Require Import coqutil.Tactics.Tactics.
+Local Open Scope Z_scope.
+
+(* Proofs about cmd.while *)
+
+Section Proofs.
+  Context {p : Semantics.parameters} {p_pk : Semantics.parameters_ok p}.
+
+  Fixpoint repeat_logic_step
+           (logic : trace -> mem -> locals ->
+                    (trace -> mem -> locals -> Prop) -> Prop)
+           (n : nat) post : trace -> mem -> locals -> Prop :=
+    match n with
+    | O => post
+    | S n => fun t m l => logic t m l (repeat_logic_step logic n post)
+    end.
+
+  Lemma unroll_while functions conde body t m l
+        (iterations : nat)
+        (post : trace -> mem -> locals -> Prop) (cond : Semantics.word) :
+    repeat_logic_step
+      (fun t m l post =>
+         exists cond,
+           dexpr m l conde cond
+           /\ word.unsigned cond <> 0
+           /\ cmd (call functions) body t m l post)
+      iterations (fun t m l =>
+                    dexpr m l conde cond
+                    /\ word.unsigned cond = 0
+                    /\ post t m l) t m l ->
+    cmd (call functions) (cmd.while conde body) t m l post.
+  Proof.
+    lazymatch goal with
+      |- repeat_logic_step ?logic _ ?post _ _ _ -> _ =>
+      set (step:=logic);
+        set (P:=post)
+    end.
+    intros. exists nat, lt, (fun i => repeat_logic_step step i P).
+    ssplit.
+    { exact lt_wf. }
+    { eauto. }
+    { intro i. destruct i; cbn [repeat_logic_step].
+      { (* i=0 case (contradiction) *)
+        subst P. repeat straightline.
+        eexists; ssplit; eauto; congruence. }
+      { (* i <> 0 case *)
+        subst step. repeat straightline.
+        eexists; ssplit; eauto; try congruence; [ ].
+        repeat straightline.
+        eapply Proper_cmd; [ apply Proper_call | | eassumption ].
+        repeat intro. exists i. ssplit; eauto. } }
+  Qed.
+End Proofs.
